

Problem 40. Prove that an abelian group has a composition series if and only if it is finite.

Proof. (\Leftarrow) If G is finite, it must have order $n = \prod_{i=1}^m p_i^{a_i}$ for some distinct primes p_1, \dots, p_m and $a_1, \dots, a_m \in \mathbb{Z}^+$. Every subgroup of G is normal since it's abelian, so each Sylow p_i -subgroup $P_i < G$ of order $p_i^{a_i}$ is normal. So by **Problem 36**, G is the internal direct product $G = P_1 \cdots P_m \cong P_1 \times \cdots \times P_m$ of its Sylow subgroups. Now consider any $a, b \in P_1 \cdots P_k \setminus P_1 \cdots P_{k-1}$ for some $1 < k \leq m$.

$$[a] = [b] \in P_1 \cdots P_k / P_1 \cdots P_{k-1} \implies b^{-1}a \in P_1 \cdots P_{k-1} \implies |b^{-1}a| \text{ divides } p_1^{a_1} \cdots p_{k-1}^{a_{k-1}}.$$

$$a, b \in P_1 \cdots P_k \setminus P_1 \cdots P_{k-1} = P_k \setminus \{e\} \text{ since } P_1 \cdots P_{k-1} \cap P_k = \{e\}.$$

So $|a|, |b| \in \{p_k^i \mid 1 \leq i \leq a_k\}$ and without loss of generality, $|a| = p_k^\alpha$, $|b| = p_k^\beta$ for some $0 \leq \alpha \leq \beta \leq a_k$. So then since G is Abelian, $|b^{-1}a|$ divides $\text{lcm}(|a|, |b|) = p_k^\beta$. So the $|b^{-1}a|$ divides p_k^β and $p_1^{a_1} \cdots p_{k-1}^{a_{k-1}}$, and since $\gcd(p_1^{a_1} \cdots p_{k-1}^{a_{k-1}}, p_k^\beta) = 1$, $|b^{-1}a|$ must in fact be 1. So $b^{-1}a = e \implies a = b$. On the other hand, $a = b \implies [a] = [b]$ by definition. Therefore, for any $a, b \in P_1 \cdots P_k \setminus P_1 \cdots P_{k-1}$:

$$[a] = [b] \in P_1 \cdots P_k / P_1 \cdots P_{k-1} \iff a = b.$$

Well, any $g \in P_1 \cdots P_k$ is either in $P_1 \cdots P_k \setminus P_1 \cdots P_{k-1}$ or it isn't, so pick some $q \in P_1 \cdots P_k \setminus P_1 \cdots P_{k-1}$.

$$[g] = \begin{cases} [q], & \text{if } g \in P_1 \cdots P_k \setminus P_1 \cdots P_{k-1} \\ [e], & \text{if } g \in P_1 \cdots P_{k-1} \end{cases}$$

Therefore, $P_1 \cdots P_k / P_1 \cdots P_{k-1} = \{[e], [q]\} \cong \mathbb{Z}_2$ is simple for each $1 < k \leq m$, and by the same sort of argument $P_1 / \{e\}$ is simple since $[a] = [b] \iff b^{-1}a \in \{e\} \iff a = b \implies P_1 / \{e\} = \{[e], [g]\}$ for any $g \in P_1 \setminus \{e\}$. So $\{e\} \triangleleft P_1 \triangleleft P_1 P_2 \triangleleft \cdots \triangleleft P_1 P_2 \cdots P_{m-1} \triangleleft P_1 P_2 \cdots P_m = G$ is a composition series. We prove the other direction on the following page.

(\implies) If an abelian group G has a composition series

$$\{e\} = H_0 \triangleleft H_1 \triangleleft \cdots \triangleleft H_{n-1} \triangleleft H_n = G$$

for some $n \in \mathbb{Z}^+$, then for each $1 \leq k \leq n$, H_k/H_{k-1} is simple and abelian. So then for any $g \in H_k$, $\langle [g] \rangle = \{e\}$ or H_k/H_{k-1} . If $\langle [g] \rangle = \{e\}$, $\forall g \in H_k/H_{k-1}$, then $H_k/H_{k-1} = \{[e]\}$, otherwise $\exists g_* \in H_k$ such that $\langle [g_*] \rangle = H_k/H_{k-1}$. In either case H_k/H_{k-1} is cyclic. Suppose H_k/H_{k-1} infinite, so $H_k/H_{k-1} \cong \mathbb{Z}$. But then H_k/H_{k-1} isn't simple since \mathbb{Z} isn't simple ($\{e\} \triangleleft 2\mathbb{Z} \triangleleft \mathbb{Z}$), a contradiction. So H_k/H_{k-1} must be a simple finite cyclic group, which implies it has prime order since $H_k \triangleright H_{k-1} \implies |H_k/H_{k-1}| > 1$. Observe.

$[H_1 : H_0] \in \mathbb{Z}^+ \implies |H_1| = |H_0|[H_1 : H_0] = (1)[H_1 : H_0] \in \mathbb{Z}^+$. Suppose $|H_k| \in \mathbb{Z}^+$ for some $1 \leq k \leq n$.

Therefore, $|H_{k+1}| = |H_k|[H_{k+1} : H_k] \in \mathbb{Z}^+$. So then $|H_m| \in \mathbb{Z}^+$ for all $0 \leq m \leq n$.

So $|H_n| = |G| \in \mathbb{Z}^+$.

Thus,

An abelian group has a composition series if and only if it is finite.

□

Problem 41. Prove that a solvable simple group is abelian.

Proof. Since G is simple, $Z(G) \trianglelefteq G$ is either $\{e\}$. Suppose $Z(G) = \{e\}$, and consider the commutator subgroup $G' = \langle a^{-1}b^{-1}ab \mid a, b \in G \rangle \trianglelefteq G$. $G' \neq \{e\}$, otherwise $a^{-1}b^{-1}ab = e, \forall a, b \in G \implies G$ is abelian $\implies Z(G) = G$, a contradiction. So $G' = G$ and $G^{(2)} = (G')' = (G)' = G' = G$. Now suppose $G^{(k)} = G$ for some $k \geq 2$. Then $G^{k+1} = (G^{(k)})' = (G)' = G' = G$. But then $G^n = G \neq \{e\}$ for all $n \in \mathbb{Z}^+$, and G isn't solvable. So $Z(G) = G$.

Thus,

A solvable simple group is abelian.

□

We now prove a lemma for **Problem 42**.

Lemma 1. Any subquotient (of subgroups normal to each other) of a consecutive quotient of derived subgroups is Abelian.

Proof. Let $G^{(k-1)} \supseteq H_1 \supseteq H_2 \supseteq \dots \supseteq H_p \supseteq \dots \supseteq H_q \supseteq \dots \supseteq H_{m-1} \supseteq H_m \supseteq G^{(k)}$ for some $k, m \in \mathbb{Z}^+$ and some $0 \leq p < q \leq m$. Well,

$$(H_p)' = \{g \in G^{(k)} \mid g = a^{-1}b^{-1}ab \text{ for } a, b \in H_p \trianglelefteq G^{(k-1)}\} \trianglelefteq G^{(k)} \implies H_p \supseteq H_q \supseteq G^{(k)} \supseteq (H_p)'.$$

So then $\forall a, b \in H_p$, $(ba)^{-1}ab = a^{-1}b^{-1}ab \in (H_p)' \leq H_q \implies (ab)H_q = (ba)H_q$. Therefore, $[a][b] = [ab] = [ba] = [b][a] \in H_p/H_q$. So H_p/H_q is abelian. □

I know now that I could have used some more theorems from class to make these proofs shorter. I was in too deep here and I derived important ideas myself by doing it this way so I'm cool with it. Apologies for the lengths though.

Problem 42. Prove that a solvable group that has a composition series is finite.

Proof. If a solvable group G with a composition series is abelian, then it is finite by **Problem 40**. Suppose such a group G is not abelian. There exists a minimal $n \in \mathbb{Z}^+$ such that $G^{(n)} = \{e\}$ since G is solvable and we have (i) the derived normal series and (ii) some composition series of G :

$$(i) \ G = G^{(0)} \supseteq G' = G^{(1)} \supseteq \dots \supseteq G^{(n-1)} \supseteq G^{(n)} = \{e\} \text{ and } (ii) \ G = H_0 \triangleright H_1 \triangleright \dots \triangleright H_{m-1} \triangleright H_m = \{e\}$$

By **Schreiers's Theorem** these normal series have an equivalent refinement, that is:

$$(1) \ G_{i,j} = G^{(i+1)}(G^{(i)} \cap H_j) \text{ for } \begin{matrix} 0 \leq j \leq n-1 \\ 0 \leq j \leq m-1 \end{matrix} \text{ and } (2) \ H_{i,j} = (G^{(i)} \cap H_j)H_{j+1} \text{ for } \begin{matrix} 0 \leq j \leq n \\ 0 \leq j \leq m-1 \end{matrix}$$

$$\implies (3) \ \begin{aligned} G &= G^0 = G_{0,0} \supseteq G_{0,1} \supseteq \dots \supseteq G_{0,m} = G' = G_{1,0} \supseteq G_{1,1} \supseteq \dots \supseteq G_{1,m} = G^{(2)} = G_{2,0} \supseteq \dots \supseteq G_{n-1,m} = G^{(n)} = G_{n,0} = \{e\}. \\ G &= H_0 = H_{0,0} \supseteq H_{1,0} \supseteq \dots \supseteq H_{n,0} = H_1 = H_{0,1} \supseteq H_{1,1} \supseteq \dots \supseteq H_{n,1} = H_2 = H_{2,0} \supseteq \dots \supseteq H_{n,m-1} = H_n = H_{0,m} = \{e\} \end{aligned}$$

$$\text{and } (4) \ G_{i,j}/G_{i,j+1} \cong H_{i,j}/H_{i+1,j}.$$

These series are normal by the **Butterfly Lemma** as stated in the class notes. Now, consider any $0 \leq k \leq n$.

We have $H_{k-1} = H_{0,k-1} \supseteq \dots \supseteq H_{n,k-1} = H_k$ and H_k is a maximal proper normal subgroup of H_{k-1} , that is:

$H_k \trianglelefteq N \trianglelefteq H_{k-1} \implies N = H_{k-1} \text{ or } N = H_k$. So then since we have a containment chain, there exists some

$0 \leq p \leq n$ such that $H_{k-1} = H_{0,k-1} = \dots = H_{p,k-1} \triangleright H_{p+1,k-1} = \dots = H_{n,k-1} = H_k$. Therefore, by (4):

$$H_{k-1}/H_k = H_{p,k-1}/H_{p+1,k-1} \cong G_{p,k-1}/G_{p,k}$$

which is abelian by **Lemma 1** since it is a subquotient of $G^{(p-1)}/G^{(p)}$. So then H_{k-1}/H_k is abelian and simple, and we proved earlier in **Problem 40** that an abelian simple group must be cyclic and finite of prime order and that if quotients of a composition series of G are finite, that G itself is finite.

Thus,

A solvable group that has a composition series is finite.

□

Problem 45. If $\mathbb{K} \supseteq \mathbb{F}$ is a field extension, $u, v \in \mathbb{F}$, v is algebraic over $\mathbb{K}(u)$, and v is transcendental over \mathbb{K} , then u is algebraic over $\mathbb{K}(v)$.

Proof. v is algebraic over $\mathbb{K}(u) \implies$ there exists a non-zero degree $n \in \mathbb{Z}^+$ polynomial $P(x) = \sum_{i=0}^n p_i(u)x^i$ over $\mathbb{K}(u)$ such that $P(v) = 0$. Let $m = \max\{\deg(p_i(x)) \mid 0 \leq i \leq n\}$. Then for each $0 \leq i \leq n$, we have that $p_i(x) = \sum_{j=0}^m a_{ij}x^j$ for some $a_{i0}, \dots, a_{im} \in \mathbb{K}$. Note that if $\deg p_i(x) < m$, $a_{i(\deg p_i(x))} = \dots = a_{im} = 0$. Observe.

$$\begin{aligned} P(v) &= \sum_{i=0}^n p_i(u)v^i = \sum_{i=0}^n \left(\sum_{j=0}^m a_{ij}u^j \right) v^i = \sum_{i=0}^n \left(\sum_{j=0}^m a_{ij}v^j u^j \right) = \sum_{i=0}^n (a_{i0}v^j + a_{i1}v^j u + \dots + a_{im}v^j u^m) \\ &= \sum_{i=0}^n a_{i0}v^j + \sum_{i=0}^n a_{i1}v^j u + \dots + \sum_{i=0}^n a_{im}v^j u^m = \sum_{j=0}^m \left(\sum_{i=0}^n a_{ij}v^j u^j \right) = \sum_{j=0}^m q_j(v)u^j = Q(u) = 0, \end{aligned}$$

$$\text{where } q_j(x) = \sum_{i=0}^n a_{ij}x^j \text{ and } Q(x) = \sum_{j=0}^m q_j(v)x^j \in \mathbb{K}(v)[x].$$

Now, by definition not all a_{ij} 's are zero, so not all $q_j(x)$'s are zero. That is, there exists some $0 \leq k \leq m$ such that $q_k(x) \neq 0 \in \mathbb{K}[x]$. Well, since v is transcendental over \mathbb{K} , $q_k(x) \neq 0 \implies q_k(v) \neq 0$; v cannot be a zero of $q_k(x)$ since it's non-zero over \mathbb{K} . Therefore, $Q(x) = \sum_{j=0}^m q_j(v)x^j \neq 0 \in \mathbb{K}(v)[x]$ and since $Q(u) = 0$, u must be algebraic over $\mathbb{K}(v)$.

Thus,

if $\mathbb{K} \supseteq \mathbb{F}$ is a field extension, $u, v \in \mathbb{F}$, v is algebraic over $\mathbb{K}(u)$, and v is transcendental over \mathbb{K} ,

then u is algebraic over $\mathbb{K}(v)$.

□

Problem 46. If $\mathbb{K} \supseteq \mathbb{F}$ is a field extension and $u \in \mathbb{F}$ is algebraic of odd degree over \mathbb{K} , then so is u^2 and $\mathbb{K}(u) = \mathbb{K}(u^2)$.

Proof. Since u is algebraic of odd degree $n = 2k + 1$ over \mathbb{K} for some $k \in \mathbb{Z}^+$,

$$\mathbb{K}[x]/\langle P(x) \rangle \cong \text{Span}\{1, x, \dots, x^{n-1}\} \cong \text{Span}\{1, u, \dots, u^{n-1}\} = \mathbb{K}(u)$$

for some monic irreducible degree n polynomial $P(x)$ over \mathbb{K} such that $p(u) = 0$. (This isomorphism is the canonical one $[f(x)] \longleftrightarrow f(u)$ where $[f(x)] = [g(x)] \longleftrightarrow f(u) = g(u)$. Therefore, $[0] = [P(x)] \longleftrightarrow 0 \implies P(u) = 0 \in \mathbb{K}(u)$. This is also just given since the extension is defined by that relation but whatever.) Obviously, $u^2 \in \mathbb{K}(u)$, so any $q(u^2)$ belongs to $\mathbb{K}(u)$ and therefore any $\frac{f(u^2)}{g(u^2)} \in \mathbb{K}(u^2)$ also belongs to $\mathbb{K}(u)$. So $\mathbb{K}(u^2) \subseteq \mathbb{K}(u)$. Additionally, u^2 must be algebraic otherwise $\mathbb{K}(u^2) \cong K(x) \supset K[x] = \text{Span}\{x^m \mid m \in \mathbb{N}\}$ is infinite dimensional and so $\mathbb{K}(u^2) \subseteq \mathbb{K}(u^2)$ implies that $\mathbb{K}(u)$ is infinite dimensional, a contradiction. Next, $P(x) = \sum_{i=0}^n a_i x^i = \sum_{i=0}^{2k+1} a_i x^i = \sum_{i=0}^k a_{2i+1} x^{2i+1} + \sum_{i=0}^k a_{2i} x^{2i} = x \sum_{i=0}^k a_{2i+1} x^{2i} + \sum_{i=0}^k a_{2i} x^{2i}$ for some $a_0, \dots, a_{2k+1} \in \mathbb{K}$. So then $P(u) = u \sum_{i=0}^k a_{2i+1} u^{2i} + \sum_{i=0}^k a_{2i} u^{2i} = 0$. Since $\sum_{i=0}^k a_{2i+1} u^{2i}$ has degree $2k < n$, u can't be a zero of it since it is degree n over \mathbb{K} . Therefore,

$$u = \frac{-\sum_{i=0}^k a_{2i} u^{2i}}{\sum_{i=0}^k a_{2i+1} u^{2i}} = \frac{-\sum_{i=0}^k a_{2i} (u^2)^i}{\sum_{i=0}^k a_{2i+1} (u^2)^i} \in \left\{ \frac{f(u^2)}{g(u^2)} \mid f(x), g(x) \in \mathbb{K}[x] \text{ and } g(u^2) \neq 0 \right\} = \mathbb{K}(u^2).$$

So then any $f(u) \in \mathbb{K}(u)$ must also belong to $\mathbb{K}(u^2)$ and $\mathbb{K}(u) \supseteq \mathbb{K}(u^2)$.

Thus,

if $\mathbb{K} \subseteq \mathbb{F}$ is a field extension and $u \in \mathbb{F}$ is algebraic of odd degree over \mathbb{K} , then so is u^2 and $\mathbb{K}(u) = \mathbb{K}(u^2)$.

□

Problem 47. Let $\mathbb{K} \supseteq \mathbb{F}$ be a field extension. If $X^n - a \in \mathbb{K}[X]$ is irreducible and $u \in \mathbb{F}$ is a root of $X^n - a$ and m divides n , then the degree of u^m over \mathbb{K} is n/m . What is the irreducible polynomial of u^m over \mathbb{K} ?

Proof. Since $u^n - a = 0$ and $m \mid n$, $n = mk$ for some $k \in \mathbb{Z}^+$ and so $u^{mk} - a = 0 \implies (u^m)^k - a = 0$, so u^m is a zero of $x^k - a \in \mathbb{K}[x]$. Now, suppose $x^k - a$ is reducible over \mathbb{K} . Then $x^k - a = f(x)g(x)$ for some non-constant polynomials $f(x), g(x) \in \mathbb{K}[x]$ such that $\deg(f(x)) = \alpha$, $\deg(g(x)) = \beta$ and $\alpha + \beta = k$. So we get that $x^n - a = (x^m)^k - a = f(x^m)g(x^m)$.

(The composition $(a \circ b)(x) = a(b(x))$ over a field \mathbb{F} can only (1) multiply $b(x)$ by itself some finite number of times and/or (2) scale $b(x)$ via \mathbb{F} and/or (3) add scalars in \mathbb{F} to $b(x)$ all of which preserve structure.)

So $f(x^m)$ and $g(x^m)$ are polynomials of degree $m\alpha > 1$, and $m\beta > 1$, respectively. But then $x^n - a$ is reducible over \mathbb{K} , a contradiction. So $x^k - a$ must be irreducible over \mathbb{K} and u^m is a zero of it.

Thus,

if $\mathbb{K} \supseteq \mathbb{F}$ is a field extension, $X^n - a \in \mathbb{K}[X]$ is irreducible, $u \in \mathbb{F}$ is a root of $X^n - a$, and m divides n , then the degree of u^m over \mathbb{K} is n/m and $x^k - a$ is the irreducible polynomial of u^m over \mathbb{K} .

□

Problem 48. Let $\mathbb{K} \supseteq R \supseteq \mathbb{F}$ be an extension of rings with \mathbb{K}, \mathbb{F} fields. If $\mathbb{K} \supseteq \mathbb{F}$ is algebraic, prove that R is a field.

Proof. Since \mathbb{K} is algebraic over \mathbb{F} , $\forall \alpha \in \mathbb{K}$ there exists a minimal non-zero polynomial $f(\alpha)$ over \mathbb{F} such that $f(\alpha) = 0$. Therefore, since $R \subseteq \mathbb{K}$, it must also be algebraic over \mathbb{F} . If $\mathbb{K} = R = \mathbb{F} = \{0\}$, they're... arguably fields but then \mathbb{K} can't be algebraic over \mathbb{F} since there are no non-zero polynomials over \mathbb{F} . So $R \neq \{0\}$ and it contains some non-zero element $r \in R \subseteq \mathbb{K}$. It has a multiplicative inverse r^{-1} in \mathbb{K} and there exists some minimal degree $n \in \mathbb{Z}^+$ polynomial $P(x) = \sum_{i=0}^n a_i x^i \in \mathbb{F}[x]$ such that $P(r) = 0$. Note that since it's irreducible and $r \neq 0$, the constant term is non-zero, otherwise it's reducible: $\sum_{i=0}^n a_i x^i = \sum_{i=1}^n a_i x^i = x(\sum_{i=0}^{n-1} a_i x^{i-1})$. Observe.

$$\begin{aligned} P(r) = \sum_{i=0}^n a_i r^i = 0 &\implies r^{-1} \left(\sum_{i=0}^n a_i r^i \right) = 0 \implies r^{-1} a_0 + \sum_{i=0}^n a_i r^{i-1} = 0 \\ \implies r^{-1} a_0 = - \sum_{i=0}^n a_i r^{i-1} &\implies r^{-1} = - \frac{1}{a_0} \sum_{i=0}^n a_i r^{i-1} \in R. \end{aligned}$$

This holds because $\mathbb{F} \subseteq R$. So then every $r \in R$ has a multiplicative inverse r^{-1} in R . So then since R has multiplicative inverses, it has unity by closure, and it is commutative with no zero divisors via $R \subseteq \mathbb{K}$, R is a field.

Thus,

if $\mathbb{K} \supseteq R \supseteq \mathbb{F}$ is an extension of rings where \mathbb{K} and \mathbb{F} are fields, and $\mathbb{K} \supseteq \mathbb{F}$ is algebraic, then R is a field.

□

Problem 49. Let $f = X^3 - 6X^2 + 9X + 3 \in \mathbb{Q}[X]$.

- (a) Prove that f is irreducible in $\mathbb{Q}[X]$.
- (b) Let u be a real root of f . Consider the extension $\mathbb{Q} \subseteq \mathbb{Q}(u)$. Express each of the following elements in terms of the basis $\{1, u, u^2\}$ of the \mathbb{Q} -vector space $\mathbb{Q}(u)$:

$$u^4, \quad u^5, \quad 3u^5 - u^4 + 2, \quad (u+1)^{-1}, \quad (u^2 - 6u + 8)^{-1}.$$

Proof. (a) 3 is prime and divides all integer coefficients of $f(x) = x^3 - 6x^2 + 9x + 3 \in \mathbb{Q}[x]$ except the leading one, and $3^2 \nmid 3$, the constant term of $f(x)$, so by **Eisenstein's Criterion** $f(x)$ is irreducible over \mathbb{Q} .

(b) Since $f(x) = x^3 - 6x^2 + 9x + 3$ is monic and irreducible over \mathbb{Q} and u is a zero of it we have

$$\mathbb{Q}[x]/\langle x^3 - 6x^2 + 9x + 3 \rangle \cong \mathbb{Q}(u) = \text{Span}\{1, u, u^2\} \text{ and } u^3 - 6u^2 + 9u + 3 = 0.$$

So then $u^3 = 6u^2 - 9u - 3$. Observe.

$$u^4 = u(u^3) = u(6u^2 - 9u - 3) = 6u^3 - 9u^2 - 3u = 6(6u^2 - 9u - 3) - 9u^2 - 3u = 27u^2 - 57u - 18.$$

$$u^5 = u(u^4) = u(27u^2 - 57u - 18) = 27u^3 - 57u^2 - 18u = 27(6u^2 - 9u - 3) - 57u^2 - 18u.$$

$$= 105u^2 - 261u - 81.$$

$$3u^5 - u^4 + 2 = 3(105u^2 - 261u - 81) - (27u^2 - 57u - 18) + 2 = 288u^2 - 726u - 223.$$

Next, we use long division to factor $f(u)$ into a multiple of $(u+1)$ and $(u^2 - 6u + 8)$ so we can solve for the using the remainder. We could have solved a system but this is easier.

$$\begin{array}{r|l}
 x^3 - 6x^2 + 9x + 3 & x+1 \\
 \hline
 -x^3 - x^2 & x^2 - 7x + 16 \\
 \hline
 -7x^2 + 9x & \\
 7x^2 + 7x & \\
 \hline
 16x + 3 & \\
 -16x - 16 & \\
 \hline
 -13 &
 \end{array}$$

So $\frac{f(u)}{u+1} = u^2 - 7u + 16 - \frac{13}{u+1} \implies f(u) = 0 = (u^2 - 7u + 16)(u+1) - 13 \implies \frac{1}{13}(u^2 - 7u + 16)(u+1) = 1$.

So $(u+1)^{-1} = \frac{1}{13}(u^2 - 7u + 16)$.

Next we solve for $(u^2 - 6u + 8)^{-1}$.

Division didn't work so we just solve a system directly. $(u^2 - 6u + 8)^{-1} = au^2 + bu + c$ for some $a, b, c \in \mathbb{Q}$.

So $(u^2 - 6u + 8)(u^2 - 6u + 8)^{-1} = (u^2 - 6u + 8)(au^2 + bu + c) = au^4 + (b - 6a)u^3 + (c - 6b + 8a)u^2 + (-6c + 8b)u + 8c = (c - a)u^2 + (-3a - b - 6c)u + (-3b + 8c) = 0u^2 + 0u + 1$.

$$\begin{pmatrix} -1 & 0 & 1 & 0 \\ -3 & -1 & -6 & 0 \\ 0 & -3 & 8 & 1 \end{pmatrix} \longrightarrow \begin{pmatrix} 1 & 0 & 0 & \frac{1}{35} \\ 0 & 1 & 0 & -\frac{9}{35} \\ 0 & 0 & 1 & \frac{1}{35} \end{pmatrix}.$$

$$\implies a = \frac{1}{35}, \quad b = -\frac{9}{35}, \quad c = \frac{1}{35}.$$

So, $(u^2 - 6u + 8)^{-1} = \frac{1}{35}(u^2 - 9u + 1)$.

□

Problem 50. Let $F = \mathbb{Q}(\sqrt{2}, \sqrt{3})$. Find $[F : \mathbb{Q}]$ and a basis of F over \mathbb{Q} .

Proof. To begin, $\sqrt{2}$ and $\sqrt{3}$ are zeros of monic irreducible polynomials $x^2 - 2$ and $x^2 - 3$, respectively, over \mathbb{Q} . So $\mathbb{Q}(\sqrt{2}) \cong \mathbb{Q}[x]/\langle x^2 - 2 \rangle \cong (\text{Span}_{\mathbb{Q}}\{1, x\} \subseteq \mathbb{Q}[x]) \cong \mathbb{Q}[x]/\langle x^2 - 3 \rangle \cong \mathbb{Q}(\sqrt{3})$. So then $\mathbb{Q}(\sqrt{2}) = \text{Span}\{1, \sqrt{2}\}$ and $\mathbb{Q}(\sqrt{3}) = \text{Span}\{1, \sqrt{3}\}$. Observe.

$$\sqrt{3} = a + b\sqrt{2} \text{ for some } a, b \in \mathbb{Q} \implies 3 = (a + b\sqrt{2})^2 = (a^2 + (2ab)\sqrt{2} + 2b^2) \notin \mathbb{Q},$$

$$\sqrt{2} = a + b\sqrt{3} \text{ for some } a, b \in \mathbb{Q} \implies 2 = (a + b\sqrt{3})^2 = (a^2 + (2ab)\sqrt{3} + 3b^2) \notin \mathbb{Q},$$

$$\sqrt{6} = a + b\sqrt{2} \text{ for some } a, b \in \mathbb{Q} \implies 6 = (a + b\sqrt{2})^2 = (a^2 + (2ab)\sqrt{2} + 2b^2) \notin \mathbb{Q},$$

$$\sqrt{6} = a + b\sqrt{3} \text{ for some } a, b \in \mathbb{Q} \implies 6 = (a + b\sqrt{3})^2 = (a^2 + (2ab)\sqrt{3} + 3b^2) \notin \mathbb{Q}.$$

All of the above are contradictions. So $1, \sqrt{2}, \sqrt{3}, \sqrt{6}$ must be linearly independent over \mathbb{Q} . Next, $\mathbb{Q}(\sqrt{2}, \sqrt{3}) = \text{Span}_{\mathbb{Q}(\sqrt{2})}\{1, \sqrt{3}\} = \{\alpha + \beta\sqrt{3} \mid \alpha, \beta \in \mathbb{Q}(\sqrt{2})\} = \{(a + b\sqrt{2}) + (c + d\sqrt{2})\sqrt{3} \mid a, b, c, d \in \mathbb{Q}\} = \{a + b\sqrt{2} + c\sqrt{3} + d\sqrt{6} \mid a, b, c, d \in \mathbb{Q}\}$. So $\{1, \sqrt{2}, \sqrt{3}, \sqrt{6}\}$ spans $\mathbb{Q}(\sqrt{2}, \sqrt{3})$ and since its elements are linearly independent over \mathbb{Q} , it must be a basis for $\mathbb{Q}(\sqrt{2}, \sqrt{3})$ over \mathbb{Q} .

Thus,

$$\{1, \sqrt{2}, \sqrt{3}, \sqrt{6}\} \text{ is a basis for } \mathbb{Q}(\sqrt{2}, \sqrt{3}) \text{ over } \mathbb{Q} \text{ and } [\mathbb{Q}(\sqrt{2}, \sqrt{3}) : \mathbb{Q}] = 4.$$

□

Problem 51. Let \mathbb{K} be a field. In the field $\mathbb{K}(X)$, let $u = X^3/(X+1)$. What is $[\mathbb{K}(X) : \mathbb{K}(u)]$?

Proof. $(\mathbb{K}(u))(x) = \left\{ \frac{f(x)}{g(x)} \mid f, g \in \mathbb{K}(u)[t] \right\}$ and then $u = \frac{x^3}{x+1} \implies u(x+1) - x^3 = ux + u - x^3 = 0 \implies x^3 - ux - u = 0$. So x is a zero of the polynomial $t^3 - ut - u$ over $\mathbb{K}(u)$. This means that the degree of x over $\mathbb{K}(u)$, or equivalently, $[\mathbb{K}(x) : \mathbb{K}(u)]$ must divide 3. Therefore, $[\mathbb{K}(x) : \mathbb{K}(u)] \in \{1, 3\}$. Suppose $[\mathbb{K}(x) : \mathbb{K}(u)] = 1$, then $\mathbb{K}(x) = \mathbb{K}(u)$ and $x = \frac{f(u)}{g(u)}$ for some $f(u), g(u) \neq 0$ coprime over $\mathbb{K}(u)$. Observe.

$$\begin{aligned} x^3 - ux - u &= \left(\frac{f(u)}{g(u)}\right)^3 - u\left(\frac{f(u)}{g(u)}\right) - u = 0 \text{ and } f(u)^3 - uf(u)g(u)^2 - ug(u)^3 = 0. \text{ So then} \\ f(u)^3 &= uf(u)g(u)^2 + ug(u)^3 = ug(u)^2(f(u) + g(u)) \\ \implies 3\deg(f(u)) &= 1 + 2\deg(g(u)) + \max\{\deg(f(u)), \deg(g(u))\}. \end{aligned}$$

Let $a = \deg(f(u)), b = \deg(g(u))$ and note that both belong to \mathbb{Z}^+ . We get the following cases:

$$\begin{aligned} \begin{cases} 3a = 1 + 2b + a \\ \text{or} \\ 3a = 1 + 2b + b \end{cases} &\implies \begin{cases} 2a = 1 + 2b \\ \text{or} \\ 3a = 1 + 3b \end{cases} \implies \begin{cases} 2(a+b) = 1 \\ \text{or} \\ 3(a+b) = 1 \end{cases} \implies \begin{cases} (a+b) = \frac{1}{2} \\ \text{or} \\ (a+b) = \frac{1}{3} \end{cases}. \end{aligned}$$

Both of the above are contradictions. So $[\mathbb{K}(x) : \mathbb{K}(u)] = 3$.

□

Problem 52. Let $\mathbb{K} \subseteq \mathbb{F}$ be a field extension. If $u, v \in \mathbb{F}$ are algebraic over \mathbb{K} of degrees m and n , respectively, then $[\mathbb{K}(u, v) : \mathbb{K}] \leq mn$. If m and n are relatively prime, then $[\mathbb{K}(u, v) : \mathbb{K}] = mn$.

Proof. $\mathbb{K}(u)$ and $\mathbb{K}(v)$ have bases $\mathcal{B}_u = \{1, \dots, u^{m-1}\}$ and $\mathcal{B}_v = \{1, \dots, v^{n-1}\}$, respectively, over \mathbb{K} . Also, $\mathbb{K}(u, v) = \text{Span}_{\mathbb{K}_u} \mathcal{B}_v = \{\sum_{i=0}^{n-1} a_i u^i \mid a_0, \dots, a_{n-1} \in \mathbb{K}(u)\} = \text{Span}_{\mathbb{K}} \mathcal{B}_u \mathcal{B}_v$. So $\mathcal{B}_u \mathcal{B}_v$ span $\mathbb{K}(u, v)$ over \mathbb{K} . Therefore, $[\mathbb{K}(u, v) : \mathbb{K}] = |\mathcal{B}_u \mathcal{B}_v| \leq |\mathcal{B}_u| |\mathcal{B}_v| = mn$.

Suppose $\gcd(m, n) = 1$. Since $\mathbb{K}(u, v) \supseteq \mathbb{K}(u) \supseteq \mathbb{K}$, by the Tower Law we have:

$$[\mathbb{K}(u, v) : \mathbb{K}] = [\mathbb{K}(u, v) : \mathbb{K}(u)] [\mathbb{K}(u) : \mathbb{K}] = [\mathbb{K}(u, v) : \mathbb{K}(v)] [\mathbb{K}(v) : \mathbb{K}].$$

Therefore, $[\mathbb{K}(u) : \mathbb{K}] = m$ and $[\mathbb{K}(v) : \mathbb{K}] = n$ both divide $[\mathbb{K}(u, v) : \mathbb{K}]$, which means it is a multiple of both m and n . Well, since $\text{lcm}(m, n) = \frac{mn}{\gcd(m, n)} = mn$ and $[\mathbb{K}(u, v) : \mathbb{K}] \leq mn$, it must be the case that in fact $[\mathbb{K}(u, v) : \mathbb{K}] = mn$.

□